Optimizations/Canonicalizations/NarrowPhase_32_64.thy
@@ -1,0 +1,430 @@
+theory NarrowPhase
+  imports
+    Common
+begin
+
+nitpick_params [sat_solver = smart, max_threads = 1, verbose=true]
+
+(*
+lemma eval_not_undef:
+  "([m,p] \<turnstile> e \<mapsto> v) \<longrightarrow> v \<noteq> UndefVal"
+  by (induction e; auto)
+*)
+
+section \<open>Optimizations for Narrow/Widen Nodes\<close>
+
+text \<open>Our first goal in this section is to explore the known (fixed) bug
+  in narrowing / widening within equality comparisons, in Issue 2011.\<close>
+
+context
+  includes bit_operations_syntax
+begin
+
+
+text \<open>Some of the CodeUtil methods from the GraalVM compiler"\<close>
+
+(*
+//    public static long signExtend(long value, int inputBits) {
+//        if (inputBits < 64) {
+//            return (value >>> inputBits - 1 & 1L) == 1L 
+//                   ? value | -1L << inputBits 
+//                   : value & ~(-1L << inputBits);
+//        } else {
+//            return value;
+//        }
+//    }
+*)
+definition CodeUtil_signExtend :: "int64 \<Rightarrow> nat \<Rightarrow> int64" where
+  "CodeUtil_signExtend value inputBits =
+    (if inputBits < 64
+     then (if ((value >>> (inputBits - 1)) AND 1) = 1
+          then value OR ((-1) << inputBits)
+          else value AND NOT((-1) << inputBits))
+     else value)"
+
+(* TODO? prove that this is equal to: 
+       (value << (64 - inputBits)) >>> (64 - inputBits)
+*)
+
+(* temporary version for 32-bit in and out. *)
+definition CodeUtil_signExtend32 :: "int32 \<Rightarrow> nat \<Rightarrow> int32" where
+  "CodeUtil_signExtend32 value inputBits =
+    (if inputBits < 64
+     then (if ((value >>> (inputBits - 1)) AND 1) = 1
+          then value OR ((-1) << inputBits)
+          else value AND NOT((-1) << inputBits))
+     else value)"
+
+(*
+//     public static long zeroExtend(long value, int inputBits) {
+//         return inputBits < 64 ? value & ~(-1L << inputBits) : value;
+//     }
+*)
+definition CodeUtil_zeroExtend :: "int64 \<Rightarrow> nat \<Rightarrow> int64" where
+  "CodeUtil_zeroExtend value inputBits =
+    (if inputBits < 64
+     then value AND NOT((-1) << inputBits)
+     else value)"
+
+(* temporary version for 32-bit in and out. *)
+definition CodeUtil_zeroExtend32 :: "int32 \<Rightarrow> nat \<Rightarrow> int32" where
+  "CodeUtil_zeroExtend32 value inputBits =
+    (if inputBits < 64
+     then value AND NOT((-1) << inputBits)
+     else value)"
+
+(*
+//     public static long narrow(long value, int resultBits) {
+//         long ret = value & mask(resultBits);
+//         return signExtend(ret, resultBits);
+//     }
+*)
+definition CodeUtil_narrow :: "int64 \<Rightarrow> nat \<Rightarrow> int64" where
+  "CodeUtil_narrow value resultBits =
+    signed_take_bit (resultBits - 1) (value AND mask resultBits)"
+
+definition CodeUtil_narrow32 :: "int32 \<Rightarrow> nat \<Rightarrow> int32" where
+  "CodeUtil_narrow32 value resultBits =
+    signed_take_bit (resultBits - 1) (value AND mask resultBits)"
+
+end
+
+lemma dummy: "(0 :: int32) + 1 = 1"
+  by simp
+
+
+subsection \<open>Example tests of the CodeUtil narrow and widen operators\<close>
+
+experiment begin
+corollary "sint(CodeUtil_signExtend 0x00FF 64) = 255" by code_simp
+corollary "sint(CodeUtil_signExtend 0x007F 8)  = 127" by code_simp
+corollary "sint(CodeUtil_signExtend 0x00FF 8)  = -1" by code_simp
+corollary "sint(CodeUtil_signExtend 0x0000 1)  = 0" by code_simp
+corollary "sint(CodeUtil_signExtend 0x0001 1)  = -1" by code_simp
+
+corollary "sint(CodeUtil_zeroExtend 0x00FF 64) = 255" by code_simp
+corollary "sint(CodeUtil_zeroExtend 0x007F 8)  = 127" by code_simp
+corollary "sint(CodeUtil_zeroExtend 0x00FF 8)  = 255" by code_simp
+corollary "sint(CodeUtil_zeroExtend 0x0000 1)  = 0" by code_simp
+corollary "sint(CodeUtil_zeroExtend 0x0001 1)  = 1" by code_simp
+
+corollary "sint(CodeUtil_narrow 0xFFFF 8) = -1" by code_simp
+corollary "sint(CodeUtil_narrow 0xFF7F 8) = 127" by code_simp
+corollary "sint(CodeUtil_narrow 0x00FF 8) = -1" by code_simp
+corollary "sint(CodeUtil_narrow 0x0000 1) = 0" by code_simp
+corollary "sint(CodeUtil_narrow 0x0001 1) = -1" by code_simp
+end
+
+
+(* nitpick demo: gives kodkod warning:
+    Kodkod warning: cannot launch SAT solver, falling back on "DefaultSAT4J" 
+
+lemma "P \<longleftrightarrow> Q"
+  nitpick
+*)
+
+phase Issue2011Phase 
+  terminating size
+begin
+
+fun isDefaultForKind :: "Value \<Rightarrow> bool" where
+  "isDefaultForKind (IntVal b val) = (val = 0)" |
+  "isDefaultForKind _ = False"
+
+value "not(-1 << 8 :: int32)"
+value "mask 7 :: int32"
+
+lemma shift_n_eq_bit_n:
+  fixes val :: \<open>'a::len word\<close>
+  shows "(and (val >>> n) 1 = 1) = bit val n"
+  by (simp add: bit_iff_and_drop_bit_eq_1 shiftr_def)
+
+declare [[show_types=true]]
+lemma neg1_shift_eq_mask:
+  fixes val :: \<open>'a::len word\<close>
+  fixes n :: nat
+  assumes "n < LENGTH('a)"
+  assumes "0 < n"
+  shows "((- 1 << n) :: 'a::len word) = not (mask n)" (is "?A = ?B")
+  by (simp add: shiftl_def)
+
+lemma take_bit_suc:
+  fixes v :: int32
+  assumes "\<not> bit v (n::nat)"
+  shows "take_bit (Suc n::nat) v = take_bit (n::nat) v"
+  by (smt (verit, best) assms bit_take_bit_iff le_eq_less_or_eq less_Suc_eq_le linorder_not_less
+         signed_take_bit_eq_if_positive signed_take_bit_take_bit take_bit_signed_take_bit)
+
+
+
+lemma narrow_reverse_pos:
+  assumes 1: "and (val32 >>> 7) 1 \<noteq> 1"
+  assumes pos: "\<not> bit val32 7"
+  assumes 4: "revKonst = and konst (not (- 1 << 8))"
+  assumes 5: "intval_narrow 32 8 (IntVal32 revKonst) = IntVal32 konst"
+  shows "IntVal32 konst = intval_narrow 32 8 (IntVal32 val32)
+        \<longleftrightarrow>
+         revKonst = val32"
+  unfolding assms intval_narrow.simps narrow_helper.simps 
+  apply (simp add: neg1_shift_eq_mask signed_take_bit_eq_if_positive[OF pos])
+proof (intro iffI)
+  assume a: "konst = take_bit 7 val32"
+(*  then have "konst = take_bit 8 val32"
+    thm take_bit_Suc_from_most
+  using assms take_bit_Suc_from_most 
+*)
+  then have 8: "and konst (mask 8) = konst"
+    using mask_eq_iff_w2p
+    by (smt (verit, ccfv_SIG) and_mask_lt_2p mask_eq_iff numeral_Bit0 numeral_less_iff one_eq_numeral_iff power_strict_increasing semiring_norm(81) take_bit_eq_mask)  
+  then have "(signed_take_bit 7 revKonst) = konst"
+    using 5 by simp
+  then have 9: "(take_bit 7 revKonst) = konst"
+    by (simp add: 4 a bit_and_iff bit_take_bit_iff signed_take_bit_eq_if_positive) 
+(*
+  then have "and revKonst (mask 8) = revKonst"
+    by (simp add: "4" shiftl_def)
+  then have 10: "and val32 (mask 8) = val32"
+    using 8 9 a by fastforce
+*)
+  show "and konst (mask 8) = val32"
+
+    using 9 10 a by fastforce
+  next
+    assume b: "and konst (mask 8) = val32"
+    then have "take_bit 8 val32 = val32"
+      by (metis and.right_idem take_bit_eq_mask)
+    then have "take_bit 7 val32 = val32"
+      using take_bit_suc pos by force 
+    then have 8: "and konst (mask 8) = konst"
+      using assms 
+      print_facts
+    then show "konst = take_bit 7 val32"
+      using b 
+    qed
+
+
+(* this is where the Issue2011 bug should appear. *)
+lemma narrow_reverse_neg:
+  assumes "and (val32 >>> 7) 1 = 1"
+  assumes neg: "bit val32 7"  (* 8-bit val32 is negative *)
+  assumes "val32 = 0xC0"     (* example value from bug report *)
+  shows "IntVal32 i32 = intval_narrow 32 8 (IntVal32 val32)
+        \<longleftrightarrow> 
+         IntVal32 (or i32 (- 1 << 8)) = (IntVal32 val32)"
+  unfolding assms intval_narrow.simps narrow_helper.simps
+  apply (simp add: neg1_shift_eq_mask signed_take_bit_eq_if_negative[OF neg])
+proof (intro iffI)
+  assume "i32 = - (64::32 word)"
+  then show "or i32 (not (mask (8::nat))) = (192::32 word)"
+    apply (code_simp; simp)
+    (* now we have: 
+           i32 = - (64::32 word) \<Longrightarrow> False
+       i.e. a contradiction.  This is not provable.
+    *)
+    oops
+
+
+
+(*
+  nitpick  
+  unfolding shift_n_eq_bit_n apply simp
+  oops
+*)
+
+lemma unfold_ex_let: "(\<exists>x. x=E \<and> P) = (let x=E in P)"
+  by force
+  
+lemma unfold_ex2_let: "(\<exists>x y. x=E \<and> P x y) = (let x=E in (\<exists>y. P x y))"
+  by force
+
+lemma unfold_ex2_ex_let: "(\<exists>y. (\<exists>x. (R x y \<and> y=E x \<and> Q x y)) \<and> P y) = (\<exists>x'. (let y=E x' in (R x' y \<and> Q x' y \<and> P y)))"
+  by metis
+
+lemma unfold_ex_bubble_out: "(P \<and> (\<exists>x. Q x) \<and> R) = (\<exists>x. (Q x \<and> P \<and> R))"
+  by auto
+
+(* TODO: make this more general, but still usable in unfolding? *)
+lemma unfold_intval_eq32: 
+  "((intval_equals (IntVal32 v1) v2 = intval_equals (IntVal32 v3) v4) \<and>
+   (intval_equals (IntVal32 v1) v2 \<noteq> UndefVal))
+   = ((v1 = un_IntVal32 v2) = (v3 = un_IntVal32 v4) \<and>
+      is_IntVal32 v2 \<and> is_IntVal32 v4)" (is "?A = (?B = ?C \<and> ?I2 \<and> ?I4)")
+  proof (intro iffI)
+    assume ?A
+    show "?B = ?C \<and> ?I2 \<and> ?I4"
+      by (smt (verit, best) Value.sel(1) \<open>intval_equals (IntVal32 (v1::32 word)) (v2::Value) = intval_equals (IntVal32 (v3::32 word)) (v4::Value) \<and> intval_equals (IntVal32 v1) v2 \<noteq> UndefVal\<close> bool_to_val.elims intval_eq32 intval_eq32_simp zero_neq_one)
+  next
+    assume "?B = ?C \<and> ?I2 \<and> ?I4"
+    show ?A
+      by (smt (verit, best) Value.collapse(1) Value.disc(1) Value.discI(1) \<open>((v1::32 word) = un_IntVal32 (v2::Value)) = ((v3::32 word) = un_IntVal32 (v4::Value)) \<and> is_IntVal32 v2 \<and> is_IntVal32 v4\<close> bool_to_val.simps(1) bool_to_val.simps(2) intval_equals.simps(1))
+  qed
+
+
+(* use context assumptions about definedness to deduce int size *)
+lemma eq_must_be_int32:
+  assumes "intval_equals (IntVal32 a) b \<noteq> UndefVal"
+  shows "(intval_equals (IntVal32 a) b = intval_equals (IntVal32 c) d)
+         = ((a = un_IntVal32 b) \<longleftrightarrow> (c = un_IntVal32 d))"
+proof (rule iffI)
+  assume 1: "(intval_equals (IntVal32 a) b = intval_equals (IntVal32 c) d)"
+  obtain bv where "b = IntVal32 bv" 
+    using assms intval_eq32 is_IntVal32_def by blast 
+  then show "(a = un_IntVal32 b) \<longleftrightarrow> (c = un_IntVal32 d)"
+    using 1 assms intval_eq32 is_IntVal32_def by fastforce 
+next
+  assume 2: "(a = un_IntVal32 b) \<longleftrightarrow> (c = un_IntVal32 d)"
+  then have 3: "bool_to_val (a = un_IntVal32 b) = bool_to_val (c = un_IntVal32 d)"
+    by simp
+  obtain bv where "b = IntVal32 bv" 
+    using assms intval_eq32 is_IntVal32_def by blast
+  then have "intval_equals (IntVal32 c) d \<noteq> UndefVal"
+    using assms sorry
+  then have "intval_equals (IntVal32 a) b = intval_equals (IntVal32 c) d"
+    using 3 assms sorry
+  
+  then show "(intval_equals (IntVal32 a) b = intval_equals (IntVal32 c) d)"
+    using 2 
+    oops
+
+
+(* we first investigate the case of narrowing from 32 to 8 bits.
+Input: Constant constant == ValueNode nonConstant
+       ConvertNode convert = (ConvertNode) nonConstant;  // actually a NarrowNode
+  TODO: add some of these side conditions:
+  if isConstantConversionSupported(convert, view, smallestCompareWidth)
+  ConstantNode newConstant = canonicalConvertConstant(constantReflection, metaAccess, 
+                                      condition, convert, constant, view);
+  i.e. {
+     if (convert.preservesOrder(condition, constant, constantReflection)) {
+        Constant reverseConverted = convert.reverse(constant, constantReflection);
+              i.e. = table.getSignExtend().foldConstant(getResultBits(), getInputBits(), constant)
+        if (reverseConverted != null && 
+            convert.convert(reverseConverted, constantReflection).equals(constant))
+                     i.e.  = narrow(reverseConverted) = constant
+      return ConstantNode.forConstant(convert.getValue().stamp(view), reverseConverted, metaAccess);
+     }
+  if newConstant != null
+  return newConstant == convert.getValue()
+*)
+optimization Issue2011_Bug:
+  "((const (IntVal32 value)) eq
+      (UnaryExpr (UnaryNarrow inBits outBits) expr))
+   \<longmapsto>
+   ((const (IntVal32 (CodeUtil_signExtend32 value outBits)))
+      eq expr)
+   when (inBits = 32 \<and> outBits = 8)"
+  apply (rule impI)
+  subgoal premises 1 
+  unfolding le_expr_def unfold_evaltree bin_eval.simps unary_eval.simps
+   apply (rule allI impI)+
+  unfolding ex_neg_all_pos unfold_ex_bubble_out
+  subgoal premises 2 for m p v x y ev
+    apply (rule exI[of _ "IntVal32 (CodeUtil_signExtend32 value outBits)"];
+           rule exI[of _ ev])
+      unfolding CodeUtil_signExtend32_def 
+      apply (simp add: 1 2 unfold_intval_eq32)
+      (* this gives two conjuncts, which are similar to above lemmas:
+1. (and (value >>> (7::nat)) (1::32 word) = (1::32 word) \<longrightarrow>
+     (value = un_IntVal32 (intval_narrow (32::nat) (8::nat) ev)) =
+     (or value (- (1::32 word) << (8::nat)) = un_IntVal32 ev) \<and>
+     is_IntVal32 (intval_narrow (32::nat) (8::nat) ev) \<and> is_IntVal32 ev)
+2.  (and (value >>> (7::nat)) (1::32 word) \<noteq> (1::32 word) \<longrightarrow>
+     (value = un_IntVal32 (intval_narrow (32::nat) (8::nat) ev)) =
+     (and value (not (- (1::32 word) << (8::nat))) = un_IntVal32 ev) \<and>
+     is_IntVal32 (intval_narrow (32::nat) (8::nat) ev) \<and> is_IntVal32 ev)
+ *)
+      print_facts
+      oops
+
+
+optimization Issue2011_Fix:
+  "(BinaryExpr BinIntegerEquals
+      (ConstantExpr (IntVal32 value))
+      (UnaryExpr (UnaryNarrow inBits outBits) expr))
+   \<longmapsto>
+   (BinaryExpr BinIntegerEquals
+      (ConstantExpr (IntVal32 (CodeUtil_zeroExtend32 value outBits)))
+      expr)
+   when (inBits = 32 \<and> outBits = 8)"
+   apply unfold_optimization
+  apply (rule impI)
+  subgoal premises 1 
+  unfolding le_expr_def unfold_evaltree bin_eval.simps unary_eval.simps
+   apply (rule allI impI)+
+  unfolding ex_neg_all_pos unfold_ex_bubble_out
+  subgoal premises 2 for m p v x y ev
+      apply (rule exI[of _ "IntVal32 (CodeUtil_zeroExtend32 value outBits)"]; rule exI[of _ ev])
+      unfolding CodeUtil_zeroExtend32_def 
+      apply (simp add: 1 2 unfold_intval_eq32)
+      apply (rule conjI)
+(* this gives two goals (first one is false, e.g. ev=0x100):
+ 1. (value = un_IntVal32 (intval_narrow (32::nat) (8::nat) ev)) =
+    (and value (not (- (1::32 word) << (8::nat))) = un_IntVal32 ev)
+ 2. is_IntVal32 (intval_narrow (32::nat) (8::nat) ev) \<and> is_IntVal32 ev
+*) 
+      print_facts
+      oops
+
+
+  
+(* other side-conditions in the code:
+  NB. 'convert' and narrowNode are the unary narrow expr.
+
+  !(narrowNode.getInputBits() > 32 && !constant.isDefaultForKind())
+   smallestCompareWidth != null && 
+     intStamp.getBits() >= smallestCompareWidth
+
+  (convert.preservesOrder(condition, constant, constantReflection))
+  // then calculate reverseConverted:
+  (reverseConverted != null && convert.convert(reverseConverted, constantReflection).equals(constant))
+
+  (ConstantExpr newConstant) is: 
+    return ConstantNode.forConstant(convert.getValue().stamp(view), reverseConverted, metaAccess);
+*)
+
+
+(*
+
+optimization e:
+  "x * (const c) \<longmapsto> x << (const n) when (n = intval_log2 c \<and> in_bounds n 0 32)"
+   apply unfold_optimization apply simp using e_intval
+  using BinaryExprE ConstantExprE bin_eval.simps(2,7) sorry
+
+
+  nitpick [unary_ints]
+  nitpick [binary_ints, bits=16]
+  But these give error: 
+    Unsupported case: representation function on "Int.int"
+
++//   && supported   // ie. (convert.stamp as IntegerStamp).getBits() >= smallestCompareWidth
++//   && let value = ((PrimitiveConstant) konstant).asLong()
++//   && let narrow = convert
++//   && let inputBits = narrow.inputBits
+# Ian: instead shift left then right
++//   && let reverseConverted = if (convert.inputBits < 64)
++//                             then if (value >>> inputBits - 1 & 1L) == 1L
++//                                  then value | -1L << inputBits
++//                                  else value & ~(-1L << inputBits)
++//                             else value
++//   && reverseConverted != null   // I don't think it can be null?
++//   && narrow.convert(reverseConverted, constantReflection).equals(konstant))
++//   && !GeneratePIC.getValue(options))
++//   && let newConstant = ConstantNode.forConstant(narrow.getValue().stamp(view), reverseConverted, metaAccess)
++//   && newConstant != null
+*)
+
+lemma negate_min32:
+  fixes y :: int32
+  assumes "y = (0x80000000 :: int32)"
+  shows "-y = (0x80000000 :: int32)"
+  using assms apply code_simp
+  by force
+
+lemma sub_min32:
+  fixes y :: int32
+  assumes "y = (0x80000000 :: int32)"
+  shows "x - y = x + y"
+  unfolding assms negate_min32
+  by simp 
+
+end
